basic generated embedding working

src/extraction/FStar.Extraction.ML.RegEmb.fst
@@ -30,6 +30,8 @@ open FStar.Syntax.Syntax
 module BU    = FStar.Compiler.Util
 module Code  = FStar.Extraction.ML.Code
 module EMB   = FStar.Syntax.Embeddings
+module Env   = FStar.TypeChecker.Env
+module N     = FStar.TypeChecker.Normalize
 module PC    = FStar.Parser.Const
 module Print = FStar.Syntax.Print
 module S     = FStar.Syntax.Syntax
@@ -40,7 +42,21 @@ module Util  = FStar.Extraction.ML.Util
 
 exception Unsupported of string
 
+let splitlast s = let x::xs = List.rev s in (List.rev xs, x)
+
 let mk e = with_ty MLTY_Top e
+
+let ml_name : Ident.lid -> mlexpr =
+  fun l ->
+    let s = Ident.path_of_lid l in
+    let ns, id = splitlast s in
+    mk (MLE_Name (ns, id))
+let ml_ctor : Ident.lid -> list mlexpr -> mlexpr =
+  fun l args ->
+    let s = Ident.path_of_lid l in
+    let ns, id = splitlast s in
+    mk (MLE_CTor ((ns, id), args))
+
 let ml_none : mlexpr = mk (MLE_Name (["FStar"; "Pervasives"; "Native"], "None"))
 let ml_some : mlexpr = mk (MLE_Name (["FStar"; "Pervasives"; "Native"], "Some"))
 
@@ -48,6 +64,28 @@ let tm_fvar_lid    = Ident.lid_of_str "FStar.Syntax.Syntax.Tm_fvar"
 let fv_eq_lid_lid  = Ident.lid_of_str "FStar.Syntax.Syntax.fv_eq_lid"
 let s_fvar_lid     = Ident.lid_of_str "FStar.Syntax.Syntax.fvar"
 let lid_of_str_lid = Ident.lid_of_str "FStar.Ident.lid_of_str" // :^)
+let mk_app_lid     = Ident.lid_of_str "FStar.Syntax.Util.mk_app"
+let nil_lid        = Ident.lid_of_str "Prims.Nil"
+let cons_lid       = Ident.lid_of_str "Prims.Cons"
+let embed_lid      = Ident.lid_of_str "FStar.Syntax.Embeddings.Base.extracted_embed"
+let unembed_lid    = Ident.lid_of_str "FStar.Syntax.Embeddings.Base.extracted_unembed"
+let bind_opt_lid   = Ident.lid_of_str "FStar.Compiler.Util.bind_opt"
+
+let ml_magic : mlexpr =
+  mk (MLE_Coerce (ml_unit, MLTY_Top, MLTY_Top))
+
+let embedding_for (a:S.typ) : mlexpr =
+  ml_magic
+
+let rec as_ml_list (ts : list mlexpr) : mlexpr =
+  match ts with
+  | [] -> ml_ctor nil_lid []
+  | t::ts -> ml_ctor cons_lid [t; as_ml_list ts]
+
+let rec pats_to_list_pat (vs : list mlpattern) : mlpattern =
+  match vs with
+  | [] -> MLP_CTor ((["Prims"], "Nil"), [])
+  | p::ps -> MLP_CTor ((["Prims"], "Cons"), [p; pats_to_list_pat ps])
 
 let fresh : string -> string =
   let r = BU.mk_ref 0 in
@@ -55,8 +93,6 @@ let fresh : string -> string =
     let v = !r in
     r := v+1;
     s^"_"^(string_of_int v)
-
-let splitlast s = let x::xs = List.rev s in (List.rev xs, x)
 
 let mk_unembed (ctors: list sigelt) : mlexpr =
   let e_branches : ref (list mlbranch) = BU.mk_ref [] in
@@ -66,15 +102,26 @@ let mk_unembed (ctors: list sigelt) : mlexpr =
     | Sig_datacon {lid; us; t; ty_lid; num_ty_params; mutuals} ->
       let fv = fresh "fv" in
       let bs, c = U.arrow_formals t in
-      (* let vs = List.map (fun b -> fresh (Ident.string_of_id b.binder_bv.ppname)) bs in *)
+      let vs = List.map (fun b -> fresh (Ident.string_of_id b.binder_bv.ppname), b.binder_bv.sort) bs in
 
       let pat_s = MLP_Const (MLC_String (Ident.string_of_lid lid)) in
-      let pat_args = MLP_CTor ((["Prims"], "Nil"), []) in
+      (* let pat_args = MLP_CTor ((["Prims"], "Nil"), List.map (fun (v, _) -> MLP_Var v) vs) in *)
+      let pat_args = vs |> List.map (fun (v,_) -> MLP_Var v) |> pats_to_list_pat in
       let pat_both = MLP_Tuple [pat_s; pat_args] in
 
-      let ret = mk (MLE_Name (splitlast (Ident.path_of_lid lid))) in
-      let ret = mk (MLE_App (ml_some, [ret])) in
-      let br = (pat_both, None, ret) in
+      let head = ml_name lid in
+      let ret = mk (MLE_App (head, [mk (MLE_Tuple (List.map (fun (v, _) -> mk (MLE_Var v)) vs))])) in
+      let ret = mk (MLE_App (ml_some, [ret])) in // final return
+
+      let body = List.fold_right (fun (v, ty) body ->
+        let body = mk (MLE_Fun ([(v, MLTY_Top)], body)) in
+        mk (MLE_App (ml_name bind_opt_lid, [
+                      mk (MLE_App (ml_name unembed_lid, [embedding_for ty; mk (MLE_Var v)]));
+                      body;
+                      ]))
+      ) vs ret
+      in
+      let br = (pat_both, None, body) in
 
       e_branches := br :: !e_branches
     | _ -> failwith "impossible, filter above"
@@ -94,15 +141,26 @@ let mk_embed (ctors: list sigelt) : mlexpr =
     | Sig_datacon {lid; us; t; ty_lid; num_ty_params; mutuals} ->
       let fv = fresh "fv" in
       let bs, c = U.arrow_formals t in
-      (* let vs = List.map (fun b -> fresh (Ident.string_of_id b.binder_bv.ppname)) bs in *)
-
-      let pat = MLP_CTor (splitlast (Ident.path_of_lid lid), []) in
-      let fvar = mk (MLE_Name (splitlast (Ident.path_of_lid s_fvar_lid))) in
-      let lid_of_str = mk (MLE_Name (splitlast (Ident.path_of_lid lid_of_str_lid))) in
-      let ret = mk (MLE_App (fvar, [
+      let vs = List.map (fun b -> fresh (Ident.string_of_id b.binder_bv.ppname), b.binder_bv.sort) bs in
+      let pat = MLP_CTor (splitlast (Ident.path_of_lid lid), List.map (fun v -> MLP_Var (fst v)) vs) in
+      let fvar = ml_name s_fvar_lid in
+      let lid_of_str = ml_name lid_of_str_lid in
+      let head = mk (MLE_App (fvar, [
                     mk (MLE_App (lid_of_str, [mk (MLE_Const (MLC_String (Ident.string_of_lid lid)))]));
                     ml_none]))
       in
+      let mk_mk_app t ts =
+        // FIXME: all explicit
+        let ts = List.map (fun t -> mk (MLE_Tuple [t; ml_none])) ts in
+        mk (MLE_App (ml_name mk_app_lid, [t; as_ml_list ts]))
+      in
+      let args =
+        vs |> List.map (fun (v, ty) ->
+          let vt = mk (MLE_Var v) in
+          mk (MLE_App (ml_name embed_lid, [embedding_for ty; vt]))
+        )
+      in
+      let ret = mk_mk_app head args in
       let br = (pat, None, ret) in
 
       e_branches := br :: !e_branches
@@ -113,6 +171,398 @@ let mk_embed (ctors: list sigelt) : mlexpr =
   let def = mk (MLE_Match (sc, branches)) in
   let lam = mk (MLE_Fun ([arg_v, MLTY_Top], def)) in
   lam
+
+(* helper functions used to extract, alongside a tactic, its corresponding call
+   to FStar.Tactics.Native.register_tactic *)
+module RC = FStar.Reflection.Constants
+module SEmb = FStar.Syntax.Embeddings
+module REmb = FStar.Reflection.Embeddings
+
+exception NoTacticEmbedding of string
+
+let not_implemented_warning r t msg =
+    Errors.log_issue r
+        (Errors.Warning_PluginNotImplemented,
+         BU.format3 "Plugin %s can not run natively because %s (use --warn_error -%s to carry on)."
+                        t
+                        msg
+                        (string_of_int <| Errors.error_number (Errors.lookup Errors.Warning_PluginNotImplemented)))
+
+type emb_loc =
+    | Syntax_term (* FStar.Syntax.Embeddings *)
+    | Refl_emb    (* FStar.Reflection.Embeddings *)
+    | NBE_t       (* FStar.TypeChecker.NBETerm *)
+    | NBERefl_emb (* FStar.Reflection.NBEEmbeddings *)
+
+type embedding_data = {
+  arity : int;
+  syn_emb : Ident.lid; (* lid for regular embedding *)
+  nbe_emb : option Ident.lid; (* nbe embedding, optional! will abort _at runtime_ if None and called *)
+}
+
+let known_embeddings : ref (list (Ident.lident * embedding_data)) =
+  let syn_emb_lid s      = Ident.lid_of_path ["FStar"; "Syntax"; "Embeddings"; s] Range.dummyRange in
+  let nbe_emb_lid s      = Ident.lid_of_path ["FStar"; "TypeChecker"; "NBETerm"; s] Range.dummyRange in
+  let refl_emb_lid s     = Ident.lid_of_path ["FStar"; "Reflection"; "Embeddings"; s] Range.dummyRange in
+  let nbe_refl_emb_lid s = Ident.lid_of_path ["FStar"; "Reflection"; "NBEEmbeddings"; s] Range.dummyRange in
+  BU.mk_ref [
+    (PC.int_lid,                          {arity=0; syn_emb=syn_emb_lid  "e_int";        nbe_emb=Some(nbe_emb_lid "e_int")});
+    (PC.bool_lid,                         {arity=0; syn_emb=syn_emb_lid  "e_bool";       nbe_emb=Some(nbe_emb_lid "e_bool")});
+    (PC.unit_lid,                         {arity=0; syn_emb=syn_emb_lid  "e_unit";       nbe_emb=Some(nbe_emb_lid "e_unit")});
+    (PC.string_lid,                       {arity=0; syn_emb=syn_emb_lid  "e_string";     nbe_emb=Some(nbe_emb_lid "e_string")});
+    (PC.norm_step_lid,                    {arity=0; syn_emb=syn_emb_lid  "e_norm_step";  nbe_emb=Some(nbe_emb_lid "e_norm_step")});
+
+    (PC.list_lid,                         {arity=1; syn_emb=syn_emb_lid  "e_list";       nbe_emb=Some(nbe_emb_lid "e_list")});
+    (PC.option_lid,                       {arity=1; syn_emb=syn_emb_lid  "e_option";     nbe_emb=Some(nbe_emb_lid "e_option")});
+    (PC.sealed_lid,                       {arity=1; syn_emb=syn_emb_lid  "e_sealed";     nbe_emb=Some(nbe_emb_lid "e_sealed")});
+
+    (PC.mk_tuple_lid 2 Range.dummyRange,  {arity=1; syn_emb=syn_emb_lid  "e_tuple2";     nbe_emb=Some(nbe_emb_lid "e_tuple2")});
+
+    (RC.fstar_refl_types_lid "term",      {arity=0; syn_emb=refl_emb_lid "e_term";      nbe_emb=Some(nbe_refl_emb_lid "e_term")});
+    (RC.fstar_refl_types_lid "fv",        {arity=0; syn_emb=refl_emb_lid "e_fv";        nbe_emb=Some(nbe_refl_emb_lid "e_fv")});
+    (RC.fstar_refl_types_lid "sigelt",    {arity=0; syn_emb=refl_emb_lid "e_sigelt";    nbe_emb=Some(nbe_refl_emb_lid "e_sigelt")});
+    (RC.fstar_refl_types_lid "env",       {arity=0; syn_emb=refl_emb_lid "e_env";       nbe_emb=Some(nbe_refl_emb_lid "e_env")});
+    (RC.fstar_refl_types_lid "binders",   {arity=0; syn_emb=refl_emb_lid "e_binders";   nbe_emb=Some(nbe_refl_emb_lid "e_binders")});
+    (RC.fstar_refl_types_lid "binder",    {arity=0; syn_emb=refl_emb_lid "e_binder";    nbe_emb=Some(nbe_refl_emb_lid "e_binder")});
+    (RC.fstar_refl_types_lid "term",      {arity=0; syn_emb=refl_emb_lid "e_term";      nbe_emb=Some(nbe_refl_emb_lid "e_term")});
+  ]
+
+let register_embedding (l: Ident.lident) (d: embedding_data) : unit =
+  known_embeddings := (l,d) :: !known_embeddings
+
+let find_embedding' (l: Ident.lident) : option embedding_data =
+  match List.find (fun (l', _) -> Ident.lid_equals l l') !known_embeddings with
+  | Some (_, data) -> Some data
+  | None -> None
+
+let find_embedding (l: Ident.lident) : embedding_data =
+  match find_embedding' l with
+  | Some data -> data
+  | None ->
+    // TODO: rename to NoEmbedding
+    raise (NoTacticEmbedding ("Embedding not defined for type " ^ Ident.string_of_lid l))
+
+type wrapped_term = mlexpr * mlexpr * int * bool
+
+let interpret_plugin_as_term_fun (env:UEnv.uenv) (fv:fv) (t:typ) (arity_opt:option int) (ml_fv:mlexpr')
+    : option wrapped_term =
+    let fv_lid = fv.fv_name.v in
+    let tcenv = UEnv.tcenv_of_uenv env in
+    let t = N.normalize [
+      Env.EraseUniverses;
+      Env.AllowUnboundUniverses;
+      Env.UnfoldUntil S.delta_constant; // unfold abbreviations such as nat
+      Env.ForExtraction
+    ] tcenv t in
+    let w = with_ty MLTY_Top in
+    let as_name mlp       = with_ty MLTY_Top <| MLE_Name mlp in
+    let lid_to_name l     = with_ty MLTY_Top <| MLE_Name (UEnv.mlpath_of_lident env l) in
+    let str_to_name s     = as_name ([], s) in
+    let fstar_tc_nbe_prefix s = as_name (["FStar_TypeChecker_NBETerm"], s) in
+    let fstar_syn_emb_prefix s = as_name (["FStar_Syntax_Embeddings"], s) in
+    let fstar_refl_emb_prefix s = as_name (["FStar_Reflection_Embeddings"], s) in
+    let fstar_refl_nbeemb_prefix s = as_name (["FStar_Reflection_NBEEmbeddings"], s) in
+    let fv_lid_embedded =
+        with_ty MLTY_Top <|
+            MLE_App (as_name (["FStar_Ident"],"lid_of_str"),
+                     [with_ty MLTY_Top <| MLE_Const (MLC_String (Ident.string_of_lid fv_lid))])
+    in
+    let emb_prefix = function
+        | Syntax_term -> fstar_syn_emb_prefix
+        | Refl_emb -> fstar_refl_emb_prefix
+        | NBE_t -> fstar_tc_nbe_prefix
+        | NBERefl_emb -> fstar_refl_nbeemb_prefix
+    in
+    let mk_tactic_interpretation l arity =
+      if arity > FStar.Tactics.InterpFuns.max_tac_arity then
+        raise (NoTacticEmbedding("tactic plugins can only take up to 20 arguments"))
+      else
+      let idroot =
+        match l with
+        | Syntax_term ->
+          "mk_tactic_interpretation_"
+        | _ ->
+          "mk_nbe_tactic_interpretation_"
+      in
+      as_name (["FStar_Tactics_InterpFuns"], idroot^string_of_int arity)
+    in
+    let mk_from_tactic l arity =
+      let idroot =
+        match l with
+        | Syntax_term -> "from_tactic_"
+        | _ -> "from_nbe_tactic_"
+      in
+      as_name (["FStar_Tactics_Native"], idroot^string_of_int arity)
+    in
+    let mk_arrow_as_prim_step l (arity: int): mlexpr =
+        emb_prefix l ("arrow_as_prim_step_" ^ string_of_int arity)
+    in
+    let mk_any_embedding l (s: string): mlexpr =
+        w <| MLE_App(emb_prefix l "mk_any_emb", [str_to_name s])
+    in
+    let mk_lam nm e =
+        w <| MLE_Fun ([(nm, MLTY_Top)], e)
+    in
+    let emb_arrow l e1 e2 =
+        w <| MLE_App(emb_prefix l "e_arrow", [e1; e2])
+    in
+    let find_env_entry bv (bv', _) = S.bv_eq bv bv' in
+    (*  Generates the ML syntax of a term of type
+           `FStar.Syntax.Embeddings.embedding [[t]]`
+        where [[t]] is the ML denotation of the F* type t
+    *)
+    let rec mk_embedding l (env:list (bv * string)) (t: term): mlexpr =
+        let t = FStar.TypeChecker.Normalize.unfold_whnf' [Env.ForExtraction] tcenv t in
+        match (FStar.Syntax.Subst.compress t).n with
+        | Tm_name bv
+             when BU.for_some (find_env_entry bv) env ->
+          mk_any_embedding l <| snd (BU.must (BU.find_opt (find_env_entry bv) env))
+
+        | Tm_refine {b=x} ->
+          (* Refinements are irrelevant to generate embeddings. *)
+          mk_embedding l env x.sort
+
+        | Tm_ascribed {tm=t} ->
+          mk_embedding l env t
+
+        | Tm_arrow {bs=[b]; comp=c} when U.is_pure_comp c ->
+          let bs, c = FStar.Syntax.Subst.open_comp [b] c in
+          let t0 = (List.hd bs).binder_bv.sort in
+          let t1 = U.comp_result c in
+          emb_arrow l (mk_embedding l env t0) (mk_embedding l env t1)
+
+        | Tm_arrow {bs=b::more::bs; comp=c} ->
+          let tail = S.mk (Tm_arrow {bs=more::bs; comp=c}) t.pos in
+          let t = S.mk (Tm_arrow {bs=[b]; comp=S.mk_Total tail}) t.pos in
+          mk_embedding l env t
+
+        | Tm_fvar _
+        | Tm_uinst _
+        | Tm_app _ ->
+          let head, args = U.head_and_args t in
+          let n_args = List.length args in
+          begin
+          match (U.un_uinst head).n with
+          | Tm_fvar fv when Some? (find_embedding' fv.fv_name.v) ->
+            let arg_embeddings =
+                args
+                |> List.map (fun (t, _) -> mk_embedding l env t)
+            in
+            let emb_data = find_embedding fv.fv_name.v in
+            let t_arity = emb_data.arity in
+            let head =
+              match l with
+              | Syntax_term -> ml_name emb_data.syn_emb
+              | NBE_t ->
+                begin match emb_data.nbe_emb with
+                | Some lid -> ml_name lid
+                | None -> ml_magic // FIXME: something better please
+                end
+              | _ -> failwith "blah"
+            in
+            if t_arity = 0
+            then head
+            else w <| MLE_App (head, arg_embeddings)
+
+          | _ ->
+            raise (NoTacticEmbedding("Embedding not defined for type " ^ (Print.term_to_string t)))
+          end
+
+        | _ ->
+          raise (NoTacticEmbedding("Embedding not defined for type " ^ (Print.term_to_string t)))
+    in
+    (* abstract_tvars:
+         body is an implicitly polymorphic function over tvar_names
+        whose type is of the form `args -> term`
+
+       returns an mlexpr that explicitly abstracts over FStar.Syntax.term
+               representations of those type arguments
+               peeling away a prefix of args corresponding to the type arguments
+     *)
+    let abstract_tvars tvar_names (body:mlexpr) : mlexpr =
+        match tvar_names with
+        | [] ->
+          let body =
+              w <| MLE_App(as_name (["FStar_Syntax_Embeddings"], "debug_wrap"),
+                            [with_ty MLTY_Top <| MLE_Const (MLC_String (Ident.string_of_lid fv_lid));
+                             mk_lam "_" (w <| MLE_App(body, [str_to_name "args"]))])
+          in
+          mk_lam "args" body
+        | _ ->
+          let args_tail = MLP_Var "args_tail" in
+          let mk_cons hd_pat tail_pat =
+              MLP_CTor ((["Prims"], "Cons"), [hd_pat; tail_pat])
+          in
+          let fst_pat v =
+              MLP_Tuple [MLP_Var v; MLP_Wild]
+          in
+          let pattern =
+              List.fold_right
+                (fun hd_var -> mk_cons (fst_pat hd_var))
+                tvar_names
+                args_tail
+          in
+          let branch =
+             pattern,
+             None,
+             w <| MLE_App(body, [as_name ([], "args")])
+          in
+          let default_branch =
+              MLP_Wild,
+              None,
+              w <| MLE_App(str_to_name "failwith",
+                            [w <| MLE_Const (MLC_String "arity mismatch")])
+          in
+          let body =
+              w <| MLE_Match(as_name ([], "args"), [branch; default_branch])
+          in
+          let body =
+              w <| MLE_App(as_name (["FStar_Syntax_Embeddings"], "debug_wrap"),
+                            [with_ty MLTY_Top <| MLE_Const (MLC_String (Ident.string_of_lid fv_lid));
+                             mk_lam "_" body])
+          in
+          mk_lam "args" body
+    in
+    (* We're trying to register a plugin or tactic
+       ml_fv which has source F* type t *)
+    let bs, c = U.arrow_formals_comp t in
+    let bs, c =
+        match arity_opt with
+        | None -> bs, c
+        | Some n ->
+          let n_bs = List.length bs in
+          if n = n_bs then bs, c
+          else if n < n_bs
+          then let bs, rest = BU.first_N n bs in
+               let c = S.mk_Total <| U.arrow rest c in
+               bs, c
+          else // n > bs
+               let msg =
+                BU.format3
+                    "Embedding not defined for %s; expected arity at least %s; got %s"
+                    (Ident.string_of_lid fv_lid)
+                    (BU.string_of_int n)
+                    (BU.string_of_int n_bs) in
+               raise (NoTacticEmbedding msg)
+    in
+    let result_typ = U.comp_result c in
+    let arity = List.length bs in
+    let type_vars, bs =
+        match
+            BU.prefix_until
+                (fun ({binder_bv=b}) ->
+                    match (SS.compress b.sort).n with
+                    | Tm_type _ -> false
+                    | _ -> true)
+               bs
+        with
+        | None ->
+          bs, []
+        | Some (tvars, x, rest) ->
+          tvars, x::rest
+    in
+    (* Explicit polymorphism in the source type `t`
+       is turned into implicit polymorphism in ML.
+
+           `t` is really `forall type_vars. bs -> result_typ`
+    *)
+    let tvar_arity = List.length type_vars in
+    let non_tvar_arity = List.length bs in
+    let tvar_names = List.mapi (fun i tv -> ("tv_" ^ string_of_int i)) type_vars in
+    let tvar_context : list (bv * string) = List.map2 (fun b nm -> b.binder_bv, nm) type_vars tvar_names in
+    // The tvar_context records all the ML type variables in scope
+    // All their embeddings will be just identity embeddings
+
+    (* aux: The main function that builds the registration code
+
+        accum_embeddings: all the embeddings of the arguments (in reverse order)
+        bs: the remaining arguments
+
+        returns (mlexpr, //the registration code
+                 int,    //the arity of the compiled code (+1 for tactics)
+                 bool)   //true if this is a tactic
+    *)
+    let rec aux loc (accum_embeddings:list mlexpr) bs : (mlexpr * int * bool) =
+        match bs with
+        | [] ->
+          let arg_unembeddings = List.rev accum_embeddings in
+          let res_embedding = mk_embedding loc tvar_context result_typ in
+          let fv_lid = fv.fv_name.v in
+          if U.is_pure_comp c
+          then begin
+            let cb = str_to_name "cb" in
+            let embed_fun_N = mk_arrow_as_prim_step loc non_tvar_arity in
+            let args = arg_unembeddings
+                    @ [res_embedding;
+                       lid_to_name fv_lid;
+                       with_ty MLTY_Top <| MLE_Const (MLC_Int(string_of_int tvar_arity, None));
+                       fv_lid_embedded;
+                       cb]
+            in
+            let fun_embedding = w <| MLE_App(embed_fun_N, args) in
+            let tabs = abstract_tvars tvar_names fun_embedding in
+            let cb_tabs = mk_lam "cb" tabs in
+            ((if loc = NBE_t then cb_tabs else mk_lam "_psc" cb_tabs),
+             arity,
+             true)
+          end
+          else if Ident.lid_equals (FStar.TypeChecker.Env.norm_eff_name tcenv (U.comp_effect_name c))
+                                    PC.effect_TAC_lid
+          then begin
+            let h = mk_tactic_interpretation loc non_tvar_arity in
+            let tac_fun = w <| MLE_App (mk_from_tactic loc non_tvar_arity,
+                                      [lid_to_name fv_lid])
+            in
+            let psc = str_to_name "psc" in
+            let ncb = str_to_name "ncb" in
+            let all_args = str_to_name "args" in
+            let args =
+                [tac_fun] @
+                arg_unembeddings @
+                [res_embedding;
+                 psc;
+                 ncb] in
+            let tabs =
+              match tvar_names with
+              | [] -> mk_lam "args" (w <| MLE_App (h, args@[all_args]))
+              | _ -> abstract_tvars tvar_names (w <| MLE_App (h, args))
+            in
+            (mk_lam "psc" (mk_lam "ncb" tabs),
+             arity + 1,
+             false)
+          end
+          else raise (NoTacticEmbedding("Plugins not defined for type " ^ Print.term_to_string t))
+
+        | ({binder_bv=b})::bs ->
+          aux loc (mk_embedding loc tvar_context b.sort::accum_embeddings) bs
+    in
+    try
+        let w, a, b = aux Syntax_term [] bs in
+        let w', _, _ = aux NBE_t [] bs in
+        Some (w, w', a, b)
+    with
+    | NoTacticEmbedding msg ->
+      not_implemented_warning (Ident.range_of_lid fv.fv_name.v)
+                              (FStar.Syntax.Print.fv_to_string fv)
+                              msg;
+      None
+
+
+
+
+
+
+
+
+
+
+
+
+
+
+
+
+
 
 let __do_handle_plugin (g: uenv) (arity_opt: option int) (se: sigelt) : list mlmodule1 =
   // BU.print2 "Got plugin with attrs = %s; arity_opt=%s"
@@ -127,7 +577,7 @@ let __do_handle_plugin (g: uenv) (arity_opt: option int) (se: sigelt) : list mlm
          let fv_lid = fv.fv_name.v in
          let fv_t = lb.lbtyp in
          let ml_name_str = MLE_Const (MLC_String (Ident.string_of_lid fv_lid)) in
-         match Util.interpret_plugin_as_term_fun g fv fv_t arity_opt ml_name_str with
+         match interpret_plugin_as_term_fun g fv fv_t arity_opt ml_name_str with
          | Some (interp, nbe_interp, arity, plugin) ->
              let register, args =
                if plugin
@@ -148,7 +598,10 @@ let __do_handle_plugin (g: uenv) (arity_opt: option int) (se: sigelt) : list mlm
       | [se] -> se
       | _ -> raise (Unsupported "mutual inductives")
     in
-    let Sig_inductive_typ {lid=tlid} = typ_sigelt.sigel in
+    let Sig_inductive_typ {lid=tlid; params=ps} = typ_sigelt.sigel in
+    if List.length ps > 0 then
+      raise (Unsupported "parameters on inductive");
+    let ns = Ident.ns_of_lid tlid in
     let name = Ident.string_of_id (List.last (Ident.ids_of_lid tlid)) in
 
     let ctors = List.filter (fun se -> match se.sigel with | Sig_datacon _ -> true | _ -> false) ses in
@@ -169,6 +622,12 @@ let __do_handle_plugin (g: uenv) (arity_opt: option int) (se: sigelt) : list mlm
       print_typ     = false;
     }
     in
+    // TODO: parameters
+    register_embedding tlid {
+      arity   = 0;
+      syn_emb = Ident.lid_of_ns_and_id ns (Ident.mk_ident ("e_"^name, Range.dummyRange));
+      nbe_emb = None;
+    };
     [MLM_Let (NonRec, [lb])]
 
   | _ -> []
@@ -207,3 +666,5 @@ let maybe_register_plugin (g:uenv) (se:sigelt) : list mlmodule1 =
         []
       | Some arity_opt ->
         do_handle_plugin g arity_opt se
+
+
